Fix errors in case studies

thys/POPLmark/POPLmark_2B.thy
@@ -45,39 +45,12 @@ lemma eta_natural:
   done
 
 (* Construction of substitution *)
-type_synonym ('tv, 'v) P = "('v \<Rightarrow> ('tv, 'v) trm) \<times> ('tv \<Rightarrow> 'tv typ)"
-
 definition VVr :: "'v::var \<Rightarrow> ('tv::var, 'v) trm" where
   "VVr \<equiv> trm_ctor \<circ> \<eta>"
 definition isVVr :: "('tv::var, 'v::var) trm \<Rightarrow> bool" where
   "isVVr x \<equiv> \<exists>a. x = VVr a"
 definition asVVr :: "('tv::var, 'v::var) trm \<Rightarrow> 'v" where
   "asVVr x \<equiv> (if isVVr x then SOME a. x = VVr a else undefined)"
-
-definition Uctor :: "('tv::var, 'v::var, 'tv, 'v, ('tv, 'v) trm \<times> (('tv, 'v) P \<Rightarrow> ('tv, 'v) trm), ('tv, 'v) trm \<times> (('tv, 'v) P \<Rightarrow> ('tv, 'v) trm)) trm_pre
-  \<Rightarrow> ('tv, 'v) P \<Rightarrow> ('tv, 'v) trm" where
-  "Uctor y p \<equiv> case p of (f1, f2) \<Rightarrow> if isVVr (trm_ctor (map_trm_pre id id id id fst fst y)) then
-    f1 (asVVr (trm_ctor (map_trm_pre id id id id fst fst y)))
-  else
-    trm_ctor (tvsubst_trm_pre f2 (map_trm_pre id id id id ((\<lambda>R. R (f1, f2)) \<circ> snd) ((\<lambda>R. R (f1, f2)) \<circ> snd) y))"
-
-definition PFVars_1 :: "('tv::var, 'v::var) P \<Rightarrow> 'tv set" where
-  "PFVars_1 p \<equiv> case p of (f1, f2) \<Rightarrow> IImsupp_1_trm f1 \<union> IImsupp_typ f2"
-definition PFVars_2 :: "('tv::var, 'v::var) P \<Rightarrow> 'v set" where
-  "PFVars_2 p \<equiv> case p of (f1, _) \<Rightarrow> IImsupp_2_trm f1"
-
-definition compSS_typ :: "('tv \<Rightarrow> 'tv) \<Rightarrow> ('tv \<Rightarrow> 'tv::var typ) \<Rightarrow> 'tv \<Rightarrow> 'tv typ" where
-  "compSS_typ g f \<equiv> permute_typ g \<circ> f \<circ> inv g"
-definition compSS_trm :: "('tv \<Rightarrow> 'tv) \<Rightarrow> ('v \<Rightarrow> 'v) \<Rightarrow> ('v \<Rightarrow> ('tv::var, 'v::var) trm) \<Rightarrow> 'v \<Rightarrow> ('tv, 'v) trm" where
-  "compSS_trm g1 g2 f \<equiv> permute_trm g1 g2 \<circ> f \<circ> inv g2"
-definition Pmap :: "('tv \<Rightarrow> 'tv) \<Rightarrow> ('v \<Rightarrow> 'v) \<Rightarrow> ('tv::var, 'v::var) P \<Rightarrow> ('tv, 'v) P" where
-  "Pmap g1 g2 p \<equiv> case p of (f1, f2) \<Rightarrow> (compSS_trm g1 g2 f1, compSS_typ g1 f2)"
-lemmas compSS_defs = compSS_typ_def compSS_trm_def
-
-definition valid_P :: "('tv::var, 'v::var) P \<Rightarrow> bool" where
-  "valid_P p \<equiv> case p of (f1, f2) \<Rightarrow>
-    |SSupp_trm f1| <o cmin |UNIV::'tv set| |UNIV::'v set|
-  \<and> |SSupp_typ f2| <o cmin |UNIV::'tv set| |UNIV::'v set|"
 
 lemma asVVr_VVr: "asVVr (VVr a) = a"
   apply (unfold asVVr_def isVVr_def)
@@ -132,29 +105,6 @@ lemma isVVr_permute:
   apply (rule exI)
   apply (rule refl)
   done
-
-lemma compSS_id0s:
-  "compSS_typ id = id"
-  "compSS_trm id id = id"
-  apply (unfold compSS_typ_def compSS_trm_def trm.permute_id0 typ.permute_id0 id_o o_id inv_id)
-  apply (unfold id_def)
-  apply (rule refl)+
-  done
-
-lemma compSS_comp0_trm:
-  fixes f1 g1::"'tyvar::var \<Rightarrow> 'tyvar" and f2 g2::"'var::var \<Rightarrow> 'var"
-  assumes g_prems: "bij g1" "|supp g1| <o cmin |UNIV::'tyvar set| |UNIV::'var set|" "bij g2" "|supp g2| <o cmin |UNIV::'tyvar set| |UNIV::'var set|"
-    and f_prems: "bij f1" "|supp f1| <o cmin |UNIV::'tyvar set| |UNIV::'var set|" "bij f2" "|supp f2| <o cmin |UNIV::'tyvar set| |UNIV::'var set|"
-  shows
-    "compSS_trm f1 f2 \<circ> compSS_trm g1 g2 = compSS_trm (f1 \<circ> g1) (f2 \<circ> g2)"
-  apply (unfold compSS_trm_def)
-  apply (subst o_inv_distrib trm.permute_comp0[symmetric], (rule supp_id_bound bij_id assms ordLess_ordLeq_trans cmin2 cmin1 card_of_Card_order)+)+
-  apply (rule ext)
-  apply (rule trans[OF comp_apply])
-  apply (unfold comp_assoc)
-  apply (rule refl)
-  done
-lemmas compSS_comp0s = typ.compSS_comp0[unfolded tvcompSS_tvsubst_typ_def compSS_typ_def[symmetric]] compSS_comp0_trm
 
 lemma IImsupp_VVrs: "f2 a \<noteq> a \<Longrightarrow> imsupp f2 \<inter> IImsupp_2_trm y = {} \<Longrightarrow> y a = VVr a"
   apply (unfold imsupp_def supp_def IImsupp_2_trm_def SSupp_trm_def tvVVr_tvsubst_trm_def tv\<eta>_trm_tvsubst_trm_def VVr_def[symmetric])
@@ -241,126 +191,14 @@ lemma IImsupp_permute_commute:
     done
   done
 
-lemma compSS_cong_id_trm:
-  fixes f1 g1::"'tyvar::var \<Rightarrow> 'tyvar" and f2 g2::"'var::var \<Rightarrow> 'var"
-  assumes g_prems: "bij g1" "|supp g1| <o cmin |UNIV::'tyvar set| |UNIV::'var set|" "bij g2" "|supp g2| <o cmin |UNIV::'tyvar set| |UNIV::'var set|"
-    and f_prems: "bij f1" "|supp f1| <o cmin |UNIV::'tyvar set| |UNIV::'var set|" "bij f2" "|supp f2| <o cmin |UNIV::'tyvar set| |UNIV::'var set|"
-  shows
-    "(\<And>a. a \<in> IImsupp_1_trm h \<Longrightarrow> f1 a = a) \<Longrightarrow> (\<And>a. a \<in> IImsupp_2_trm h \<Longrightarrow> f2 a = a) \<Longrightarrow> compSS_trm f1 f2 h = h"
-  apply (unfold compSS_trm_def)
-  subgoal premises prems
-    apply (subst IImsupp_permute_commute)
-          apply (rule assms cmin1 cmin2 card_of_Card_order ordLess_ordLeq_trans)+
-    (* REPEAT_DETERM *)
-      apply (rule trans[OF Int_commute])
-      apply (rule disjointI)
-      apply (drule prems)
-      apply (erule bij_id_imsupp[rotated])
-      apply (rule assms)
-    (* repeated *)
-      apply (rule trans[OF Int_commute])
-      apply (rule disjointI)
-      apply (drule prems)
-      apply (erule bij_id_imsupp[rotated])
-      apply (rule assms)
-    (* END REPEAT_DETERM *)
-    apply (unfold comp_assoc)
-    apply (subst inv_o_simp2)
-     apply (rule assms)
-    apply (rule o_id)
-    done
-  done
-
-lemmas compSS_cong_ids = typ.compSS_cong_id[unfolded tvcompSS_tvsubst_typ_def compSS_typ_def[symmetric]] compSS_cong_id_trm
 lemmas SSupp_naturals = typ.SSupp_natural trm.SSupp_natural
 lemmas IImsupp_naturals = typ.IImsupp_natural trm.IImsupp_natural
-
-(* Recursor axioms *)
-lemma Pmap_id0: "Pmap id id = id"
-  apply (rule ext)
-  apply (unfold Pmap_def case_prod_beta compSS_id0s)
-  apply (unfold id_def prod.collapse)
-  apply (rule refl)
-  done
-
-lemma Pmap_comp0:
-  fixes f1 g1::"'tyvar::var \<Rightarrow> 'tyvar" and f2 g2::"'var::var \<Rightarrow> 'var"
-  assumes g_prems: "bij g1" "|supp g1| <o cmin |UNIV::'tyvar set| |UNIV::'var set|" "bij g2" "|supp g2| <o cmin |UNIV::'tyvar set| |UNIV::'var set|"
-    and f_prems: "bij f1" "|supp f1| <o cmin |UNIV::'tyvar set| |UNIV::'var set|" "bij f2" "|supp f2| <o cmin |UNIV::'tyvar set| |UNIV::'var set|"
-  shows
-    "Pmap f1 f2 \<circ> Pmap g1 g2 = Pmap (f1 \<circ> g1) (f2 \<circ> g2)"
-  apply (rule ext)
-  apply (unfold Pmap_def case_prod_beta)
-  apply (rule trans[OF comp_apply])
-  apply (unfold prod.inject fst_conv snd_conv)
-  apply (rule conjI bij_id supp_id_bound assms ordLess_ordLeq_trans cmin1 card_of_Card_order
-      trans[OF comp_apply[symmetric] fun_cong[OF compSS_comp0s(1)]]
-      trans[OF comp_apply[symmetric] fun_cong[OF compSS_comp0s(2)]]
-      )+
-  done
-
-lemma valid_Pmap:
-  fixes f1::"'tyvar::var \<Rightarrow> 'tyvar" and f2::"'var::var \<Rightarrow> 'var"
-  assumes f_prems: "bij f1" "|supp f1| <o cmin |UNIV::'tyvar set| |UNIV::'var set|" "bij f2" "|supp f2| <o cmin |UNIV::'tyvar set| |UNIV::'var set|"
-  shows "valid_P p \<Longrightarrow> valid_P (Pmap f1 f2 p)"
-  apply (unfold valid_P_def Pmap_def case_prod_beta compSS_defs fst_conv snd_conv)
-  apply (erule conj_forward)+
-   apply (subst SSupp_naturals; (assumption | rule assms cmin1 cmin2 card_of_Card_order ordLeq_ordLess_trans[OF card_of_image] ordLess_ordLeq_trans)+)+
-  done
-
-lemma PFVars_Pmaps:
-  fixes f1::"'tyvar::var \<Rightarrow> 'tyvar" and f2::"'var::var \<Rightarrow> 'var"
-  assumes f_prems: "bij f1" "|supp f1| <o cmin |UNIV::'tyvar set| |UNIV::'var set|" "bij f2" "|supp f2| <o cmin |UNIV::'tyvar set| |UNIV::'var set|"
-  shows "PFVars_1 (Pmap f1 f2 p) = f1 ` PFVars_1 p"
-    "PFVars_2 (Pmap f1 f2 p) = f2 ` PFVars_2 p"
-  subgoal
-    apply (unfold PFVars_1_def Pmap_def case_prod_beta fst_conv snd_conv compSS_defs)
-    apply (subst IImsupp_naturals, (rule assms cmin1 cmin2 card_of_Card_order ordLess_ordLeq_trans)+)+
-    apply (unfold image_Un)?
-    apply (rule refl)
-    done
-  subgoal
-    apply (unfold PFVars_2_def Pmap_def case_prod_beta fst_conv snd_conv compSS_defs)
-    apply (subst IImsupp_naturals, (rule assms cmin1 cmin2 card_of_Card_order ordLess_ordLeq_trans)+)+
-    apply (unfold image_Un)?
-    apply (rule refl)
-    done
-  done
-
-lemma Pmap_cong_id:
-  fixes f1::"'tyvar::var \<Rightarrow> 'tyvar" and f2::"'var::var \<Rightarrow> 'var"
-  assumes f_prems: "bij f1" "|supp f1| <o cmin |UNIV::'tyvar set| |UNIV::'var set|" "bij f2" "|supp f2| <o cmin |UNIV::'tyvar set| |UNIV::'var set|"
-  shows "(\<And>a. a \<in> PFVars_1 p \<Longrightarrow> f1 a = a) \<Longrightarrow> (\<And>a. a \<in> PFVars_2 p \<Longrightarrow> f2 a = a) \<Longrightarrow> Pmap f1 f2 p = p"
-  apply (unfold PFVars_1_def PFVars_2_def Pmap_def case_prod_beta)
-  subgoal premises prems
-    apply (subst compSS_cong_ids, (rule f_prems prems cmin1 cmin2 card_of_Card_order ordLess_ordLeq_trans | erule UnI2 UnI1 | rule UnI1)+)+
-    apply assumption
-    apply (unfold prod.collapse)
-    apply (rule refl)
-    done
-  done
 
 lemmas Cinfinite_UNIV = conjI[OF trm_pre.UNIV_cinfinite card_of_Card_order]
 lemmas Cinfinite_card = cmin_Cinfinite[OF Cinfinite_UNIV Cinfinite_UNIV]
 lemmas regularCard_card = cmin_regularCard[OF trm_pre.var_regular trm_pre.var_regular Cinfinite_UNIV Cinfinite_UNIV]
 lemmas Un_bound = regularCard_Un[OF conjunct2[OF Cinfinite_card] conjunct1[OF Cinfinite_card] regularCard_card]
 lemmas UN_bound = regularCard_UNION[OF conjunct2[OF Cinfinite_card] conjunct1[OF Cinfinite_card] regularCard_card]
-
-lemma small_PFVarss:
-  "valid_P p \<Longrightarrow> |PFVars_1 (p::('tyvar::var, 'var::var) P)| <o cmin |UNIV::'tyvar set| |UNIV::'var set|"
-  "valid_P p \<Longrightarrow> |PFVars_2 p| <o cmin |UNIV::'tyvar set| |UNIV::'var set|"
-  subgoal
-    apply (unfold PFVars_1_def case_prod_beta IImsupp_1_trm_def IImsupp_2_trm_def IImsupp_typ_def comp_def valid_P_def)
-    apply (erule conjE)+
-        apply (assumption | rule Un_bound UN_bound ordLeq_ordLess_trans[OF card_of_image] typ.set_bd_UNIV trm.FVars_bd_UNIVs cmin_greater card_of_Card_order)+
-    done
-  (* copied from above *)
-  subgoal
-    apply (unfold PFVars_2_def case_prod_beta IImsupp_1_trm_def IImsupp_2_trm_def IImsupp_typ_def comp_def valid_P_def)
-    apply (erule conjE)+
-        apply (assumption | rule Un_bound UN_bound ordLeq_ordLess_trans[OF card_of_image] typ.set_bd_UNIV trm.FVars_bd_UNIVs cmin_greater card_of_Card_order)+
-    done
-  done
 
 lemma sets_tvsubst_trm_pre:
   "set2_trm_pre (tvsubst_trm_pre f x) = set2_trm_pre x"
@@ -390,300 +228,6 @@ lemma FVars_tvsubst_typ_cmin:
   shows "FVars_typ (tvsubst_typ g x) = \<Union>((FVars_typ \<circ> g) ` FVars_typ x)"
   apply (rule FVars_tvsubst_typ)
   using assms cmin1 ordLess_ordLeq_trans by blast
-
-lemma FTVars_subset: "valid_P p \<Longrightarrow> set3_trm_pre y \<inter> PFVars_1 p = {} \<Longrightarrow>
-  (\<And>t pu p. valid_P p \<Longrightarrow> (t, pu) \<in> set5_trm_pre y \<union> set6_trm_pre y \<Longrightarrow> FTVars (pu p) \<subseteq> FTVars t \<union> PFVars_1 p) \<Longrightarrow>
-  FTVars (Uctor y p) \<subseteq> FTVars (trm_ctor (map_trm_pre id id id id fst fst y)) \<union> PFVars_1 p"
-  apply (frule iffD1[OF meta_eq_to_obj_eq[OF valid_P_def]])
-  apply (unfold case_prod_beta)
-  apply (erule conjE)+
-  subgoal premises prems
-    apply (unfold Uctor_def case_prod_beta)
-    apply (rule case_split)
-     apply (subst if_P)
-      apply assumption
-     apply (unfold isVVr_def)[1]
-     apply (erule exE)
-     apply (drule sym)
-    apply (erule subst)
-     apply (unfold asVVr_VVr)
-     apply (rule case_split[of "_ = _"])
-      apply (rule iffD2[OF arg_cong2[OF _ refl, of _ _ "(\<subseteq>)"]])
-       apply (rule arg_cong[of _ _ FTVars])
-       apply assumption
-      apply (rule Un_upper1)
-     apply (rule subsetI)
-     apply (rule UnI2)
-     apply (unfold PFVars_1_def case_prod_beta IImsupp_1_trm_def SSupp_trm_def tvVVr_tvsubst_trm_def tv\<eta>_trm_tvsubst_trm_def VVr_def[symmetric] image_comp[unfolded comp_def])[1]
-     apply (unfold comp_def)[1]
-     apply (rule UnI1)
-     apply (rule UN_I)
-      apply (rule CollectI)
-      apply assumption
-     apply assumption
-    apply (unfold if_not_P)
-    apply (erule thin_rl)
-
-    apply (unfold prod.collapse trm.FVars_ctor sets_tvsubst_trm_pre)
-    apply (subst map_subst)
-      apply (rule prems(5))
-    apply simp
-    apply (subst trm_pre.set_map, (rule bij_id supp_id_bound)+)+
-    apply (unfold image_id image_comp comp_def prod.collapse)
-    apply (rule Un_mono')+
-    subgoal
-      apply (unfold set1_trm_pre_def tvsubst_trm_pre_def PFVars_1_def UN_empty
-        sum.set_map UN_single UN_singleton UN_empty2 Un_empty_right Un_empty_left prod.set_map tvsubst_trm_pre_def
-        comp_def Abs_trm_pre_inverse[OF UNIV_I] IImsupp_1_trm_def IImsupp_typ_def SSupp_typ_def fst_conv snd_conv
-        tvVVr_tvsubst_typ_def tv\<eta>_typ_tvsubst_typ_def TyVar_def[symmetric] map_trm_pre_def typ.map_id0
-        SSupp_trm_def tvVVr_tvsubst_trm_def tv\<eta>_trm_tvsubst_trm_def VVr_def[symmetric] typ.set_map
-      )
-      using prems(4,5) apply (auto split: sum.splits simp: FVars_tvsubst_typ_cmin)
-        apply (metis singletonD typ.set(1))
-        apply (metis singletonD typ.set(1))
-       apply (metis singletonD typ.set(1))
-      apply (subst (asm) PTVars_tvsubst_pat; (auto intro: ordLess_ordLeq_trans[OF _ cmin1])?)
-       apply (metis singletonD typ.set(1))
-      done
-    apply (rule iffD2[OF arg_cong2[OF refl, of _ _ "(\<subseteq>)"]])
-      apply (rule Diff_Un_disjunct)
-      apply (rule prems)
-     apply (rule Diff_mono[OF _ subset_refl])
-     apply (unfold UN_extend_simps(2))
-      (* REPEAT_DETERM *)
-     apply (rule subset_If)
-      apply (unfold UN_empty')[1]
-      apply (rule empty_subsetI)
-     apply (rule UN_mono[OF subset_refl])
-     apply (rule prems)
-      apply (rule prems)
-     apply (unfold prod.collapse)
-     apply (erule UnI2 UnI1)
-    (* repeated *)
-     apply (rule subset_If)
-      apply (unfold UN_empty')[1]
-      apply (rule empty_subsetI)
-     apply (rule UN_mono[OF subset_refl])
-     apply (rule prems)
-      apply (rule prems)
-     apply (unfold prod.collapse)
-     apply (erule UnI2 UnI1)
-    (* END REPEAT_DETERM *)
-    done
-  done
-
-lemma FVars_subset: "valid_P p \<Longrightarrow> set4_trm_pre y \<inter> PFVars_2 p = {} \<Longrightarrow>
-  (\<And>t pu p. valid_P p \<Longrightarrow> (t, pu) \<in> set5_trm_pre y \<union> set6_trm_pre y \<Longrightarrow> FVars (pu p) \<subseteq> FVars t \<union> PFVars_2 p) \<Longrightarrow>
-  FVars (Uctor y p) \<subseteq> FVars (trm_ctor (map_trm_pre id id id id fst fst y)) \<union> PFVars_2 p"
-  apply (frule iffD1[OF meta_eq_to_obj_eq[OF valid_P_def]])
-  apply (unfold case_prod_beta)
-  apply (erule conjE)+
-  subgoal premises prems
-    apply (unfold Uctor_def case_prod_beta)
-    apply (rule case_split)
-     apply (subst if_P)
-      apply assumption
-     apply (unfold isVVr_def)[1]
-     apply (erule exE)
-     apply (drule sym)
-    apply (erule subst)
-     apply (unfold asVVr_VVr)
-     apply (rule case_split[of "_ = _"])
-      apply (rule iffD2[OF arg_cong2[OF _ refl, of _ _ "(\<subseteq>)"]])
-       apply (rule arg_cong[of _ _ FVars])
-       apply assumption
-      apply (rule Un_upper1)
-     apply (rule subsetI)
-     apply (rule UnI2)
-     apply (unfold PFVars_2_def case_prod_beta IImsupp_2_trm_def SSupp_trm_def tvVVr_tvsubst_trm_def tv\<eta>_trm_tvsubst_trm_def VVr_def[symmetric] image_comp[unfolded comp_def])[1]
-    apply (rule UnI2)
-     apply (rule UN_I)
-      apply (rule CollectI)
-      apply assumption
-     apply (unfold comp_def)[1]
-     apply assumption
-    apply (unfold if_not_P)
-    apply (erule thin_rl)
-
-    apply (unfold trm.FVars_ctor prod.collapse sets_tvsubst_trm_pre map_subst)
-    apply (subst trm_pre.set_map, (rule bij_id supp_id_bound)+)+
-    apply (unfold image_id image_comp comp_def prod.collapse sets_tvsubst_trm_pre)
-    apply (rule Un_mono')+
-      apply (rule Un_upper1)
-    apply (rule iffD2[OF arg_cong2[OF refl, of _ _ "(\<subseteq>)"]])
-      apply (rule Diff_Un_disjunct)
-      apply (rule prems)
-     apply (rule Diff_mono[OF _ subset_refl])
-     apply (unfold UN_extend_simps(2))
-      (* REPEAT_DETERM *)
-     apply (rule subset_If)
-      apply (unfold UN_empty')[1]
-      apply (rule empty_subsetI)
-     apply (rule UN_mono[OF subset_refl])
-     apply (rule prems)
-      apply (rule prems)
-     apply (unfold prod.collapse)
-     apply (erule UnI2 UnI1)
-    (* repeated *)
-     apply (rule subset_If)
-      apply (unfold UN_empty')[1]
-      apply (rule empty_subsetI)
-     apply (rule UN_mono[OF subset_refl])
-     apply (rule prems)
-      apply (rule prems)
-     apply (unfold prod.collapse)
-     apply (erule UnI2 UnI1)
-    (* END REPEAT_DETERM *)
-    done
-  done
-
-lemma permute_Uctor:
-  fixes f1::"'tv::var \<Rightarrow> 'tv" and f2::"'v::var \<Rightarrow> 'v"
-  shows "valid_P p \<Longrightarrow> bij f1 \<Longrightarrow> |supp f1| <o cmin |UNIV::'tv set| |UNIV::'v set| \<Longrightarrow> bij f2 \<Longrightarrow> |supp f2| <o cmin |UNIV::'tv set| |UNIV::'v set|
-  \<Longrightarrow> permute_trm f1 f2 (Uctor y p) = Uctor (map_trm_pre f1 f2 f1 f2
-    (\<lambda>(t, pu). (permute_trm f1 f2 t, \<lambda>p. if valid_P p then permute_trm f1 f2 (pu (Pmap (inv f1) (inv f2) p)) else undefined))
-    (\<lambda>(t, pu). (permute_trm f1 f2 t, \<lambda>p. if valid_P p then permute_trm f1 f2 (pu (Pmap (inv f1) (inv f2) p)) else undefined))
-  y) (Pmap f1 f2 p)"
-  apply (frule iffD1[OF meta_eq_to_obj_eq[OF valid_P_def]])
-  apply (subst (asm) case_prod_beta)
-  apply (erule conjE)+
-  apply (unfold Uctor_def)
-  apply (subst trm_pre.map_comp, (assumption | rule supp_id_bound bij_id ordLess_ordLeq_trans cmin1 cmin2 card_of_Card_order)+)+
-  apply (unfold id_o_commute[of f1] id_o_commute[of f2] fst_o_f comp_assoc comp_def[of snd] snd_conv case_prod_beta prod.collapse)
-  apply (subst trm_pre.map_comp[symmetric], (assumption | rule supp_id_bound bij_id ordLess_ordLeq_trans cmin1 cmin2 card_of_Card_order)+)+
-  apply (subst trm.permute_ctor[symmetric] isVVr_permute, (assumption | rule ordLess_ordLeq_trans cmin1 cmin2 card_of_Card_order)+)+
-
-  apply (rule case_split)
-   apply (subst if_P)
-    apply assumption
-   apply (unfold if_P if_not_P)
-   apply (unfold isVVr_def)[1]
-   apply (erule exE)
-   apply (erule subst[OF sym])
-   apply (subst permute_VVr)
-       apply (assumption | rule ordLess_ordLeq_trans cmin1 cmin2 card_of_Card_order)+
-   apply (unfold Pmap_def case_prod_beta fst_conv snd_conv asVVr_VVr compSS_trm_def comp_def)[1]
-   apply (subst inv_simp1)
-    apply assumption
-   apply (rule refl)
-
-  apply (rule trans)
-   apply (rule trm.permute_ctor)
-      apply (assumption | rule ordLess_ordLeq_trans cmin1 cmin2 card_of_Card_order)+
-  apply (subst map_subst)
-    apply assumption
-  apply simp
-
-  apply (subst trm_pre.map_comp, (assumption | rule supp_id_bound bij_id ordLess_ordLeq_trans cmin1 cmin2 card_of_Card_order)+)+
-  apply (unfold id_o o_id)
-  apply (unfold comp_def)
-  apply (subst if_P inv_o_simp1 trans[OF comp_apply[symmetric] Pmap_comp0[THEN fun_cong]], (rule valid_Pmap bij_imp_bij_inv supp_inv_bound | assumption)+)+
-  apply (unfold trans[OF Pmap_id0[THEN fun_cong] id_apply])
-  apply (unfold Pmap_def case_prod_beta snd_conv compSS_typ_def)
-  apply (rule arg_cong[of _ _ trm_ctor])
-
-  apply (unfold tvsubst_trm_pre_def map_trm_pre_def comp_def typ.map_id0 Abs_trm_pre_inverse[OF UNIV_I])
-  apply (frule ordLess_ordLeq_trans)
-   apply (rule cmin1 card_of_Card_order)+
-  apply (rotate_tac -3)
-  apply (unfold typ.vvsubst_permute)
-  apply (frule ordLess_ordLeq_trans)
-   apply (rule cmin1 card_of_Card_order)+
-  using typ.SSupp_natural[of f1 "snd p"] SSupp_typ_TyVar_comp[of f1]
-    SSupp_typ_tvsubst_typ_bound[of "TyVar o f1" "snd p"]
-    SSupp_typ_tvsubst_typ_bound[of "permute_typ f1 o snd p o inv f1" "TyVar o f1"]
-  apply (auto split: sum.splits simp: Abs_trm_pre_inject trans[OF comp_apply[symmetric] typ.tvsubst_permutes[THEN fun_cong]] comp_def
-      vvsubst_pat_tvsubst_pat)
-  apply (subst (1 2) tvsubst_pat_comp)
-       apply (auto simp: o_def intro!: tvsubst_pat_cong)
-    apply (meson card_of_image ordLeq_ordLess_trans)
-  using ordLeq_ordLess_trans[of "|SSupp_typ (\<lambda>uub. permute_typ f1 (snd p (inv f1 uub)))|"
-      "|SSupp_typ (snd p)|" "|top|"]
-   apply force
-  apply (subst typ.subst)
-   apply (auto simp: permute_typ_eq_tvsubst_typ_TyVar o_def)
-   apply (meson card_of_image ordLeq_ordLess_trans)
-  done
-
-ML \<open>
-val nvars: int = 2
-val parameters = {
-  P = @{typ "('tv::var, 'v::var) P"},
-  Pmap = @{term "Pmap :: _ \<Rightarrow> _ \<Rightarrow> _ \<Rightarrow> ('tv::var, 'v::var) P"},
-  PFVarss = [
-    @{term "PFVars_1 :: ('tv::var, 'v::var) P \<Rightarrow> _"},
-    @{term "PFVars_2 :: ('tv::var, 'v::var) P \<Rightarrow> _"}
-  ],
-  avoiding_sets = [@{term "{} :: 'tv::var set"}, @{term "{} :: 'v::var set"}],
-  min_bound = true,
-  validity = SOME {
-    pred = @{term "valid_P :: ('tv::var, 'v::var) P \<Rightarrow> _"},
-    valid_Pmap = fn ctxt => HEADGOAL (resolve_tac ctxt @{thms valid_Pmap} THEN_ALL_NEW assume_tac ctxt)
-  },
-  axioms = {
-    Pmap_id0 = fn ctxt => EVERY1 [
-      resolve_tac ctxt [trans],
-      resolve_tac ctxt @{thms fun_cong[OF Pmap_id0]},
-      resolve_tac ctxt @{thms id_apply}
-    ],
-    Pmap_comp0 = fn ctxt => resolve_tac ctxt @{thms fun_cong[OF Pmap_comp0[symmetric]]} 1 THEN REPEAT_DETERM (assume_tac ctxt 1),
-    Pmap_cong_id = fn ctxt => resolve_tac ctxt @{thms Pmap_cong_id} 1 THEN REPEAT_DETERM (assume_tac ctxt 1 ORELSE Goal.assume_rule_tac ctxt 1),
-    PFVars_Pmaps = replicate nvars (fn ctxt => resolve_tac ctxt @{thms PFVars_Pmaps} 1 THEN REPEAT_DETERM (assume_tac ctxt 1)),
-    small_PFVarss = replicate nvars (fn ctxt => resolve_tac ctxt @{thms small_PFVarss} 1 THEN assume_tac ctxt 1),
-    small_avoiding_sets = replicate nvars (fn ctxt => HEADGOAL (resolve_tac ctxt @{thms cmin_greater}
-      THEN_ALL_NEW resolve_tac ctxt @{thms card_of_Card_order emp_bound}))
-  }
-} : (Proof.context -> tactic) MRBNF_Recursor.parameter;
-\<close>
-
-ML \<open>
-val fp_res = the (MRBNF_FP_Def_Sugar.fp_result_of @{context} "POPLmark_2B.trm")
-val quot = hd (#quotient_fps fp_res);
-val vars = map TVar (rev (Term.add_tvarsT (#T quot) []));
-\<close>
-
-ML \<open>
-val model = MRBNF_Recursor.mk_quotient_model quot (vars ~~ [@{typ "'tv::var"}, @{typ "'v::var"}]) [] {
-  binding = @{binding "tvsubst"},
-  Uctor = @{term "Uctor :: _ \<Rightarrow> ('tv::var, 'v::var) P \<Rightarrow> _"},
-  validity = NONE,
-  axioms = {
-    FVars_subsets = [
-      fn ctxt => EVERY1 [
-        K (Local_Defs.unfold0_tac ctxt @{thms Un_empty_right}),
-        resolve_tac ctxt @{thms FTVars_subset},
-        REPEAT_DETERM o assume_tac ctxt,
-        Goal.assume_rule_tac ctxt
-      ],
-      fn ctxt => EVERY1 [
-        K (Local_Defs.unfold0_tac ctxt @{thms Un_empty_right}),
-        resolve_tac ctxt @{thms FVars_subset},
-        REPEAT_DETERM o assume_tac ctxt,
-        Goal.assume_rule_tac ctxt
-      ]
-    ],
-    permute_Uctor = fn ctxt => HEADGOAL (resolve_tac ctxt @{thms permute_Uctor} THEN_ALL_NEW assume_tac ctxt)
-  }
-}
-\<close>
-
-local_setup \<open>fn lthy =>
-let
-  val qualify = I
-  val (ress, lthy) = MRBNF_Recursor.create_binding_recursor qualify fp_res parameters [model] lthy
-  val notes =
-    [ ("rec_Uctor", map (Local_Defs.unfold0 lthy @{thms Un_empty_right} o #rec_Uctor) ress)
-    ] |> (map (fn (thmN, thms) =>
-      ((Binding.qualify true "trm" (Binding.name thmN), []), [(thms, [])])
-    ));
-  val (_, lthy) = Local_Theory.notes notes lthy
-  val _ = @{print} ress
-in lthy end
-\<close>
-print_theorems
-
-definition tvsubst :: "('v \<Rightarrow> ('tv::var, 'v::var) trm) \<Rightarrow> ('tv \<Rightarrow> 'tv typ) \<Rightarrow> ('tv, 'v) trm \<Rightarrow> ('tv, 'v) trm" where
-  "tvsubst f1 f2 t \<equiv> ff0_tvsubst t (f1, f2)"
 
 type_synonym ('tv, 'v) U1_pre = "('tv, 'v, 'tv, 'v, ('tv, 'v) trm, ('tv, 'v) trm) trm_pre"
 
@@ -817,17 +361,206 @@ lemma eta_set_empties:
     done
   done
 
-lemma tvsubst_VVr:
-  assumes
-    "|SSupp_trm f1| <o cmin |UNIV::'tv set| |UNIV::'v set|"
-    "|SSupp_typ f2| <o cmin |UNIV::'tv set| |UNIV::'v set|"
-  shows "tvsubst f1 f2 (VVr a :: ('tv::var, 'v::var) trm) = f1 a"
+context
+  fixes \<rho>1::"'v \<Rightarrow> ('tv::var, 'v::var) trm" and \<rho>2::"'tv \<Rightarrow> 'tv typ"
+  assumes f_prems: "|SSupp_trm \<rho>1| <o cmin |UNIV::'tv set| |UNIV::'v set|" "|SSupp_typ \<rho>2| <o cmin |UNIV::'tv set| |UNIV::'v set|"
+begin
+
+interpretation tvsubst: QREC_cmin_fixed_trm "IImsupp_1_trm \<rho>1 \<union> IImsupp_typ \<rho>2" "IImsupp_2_trm \<rho>1"
+  "\<lambda>y. if isVVr (trm_ctor (map_trm_pre id id id id fst fst y)) then
+    \<rho>1 (asVVr (trm_ctor (map_trm_pre id id id id fst fst y)))
+  else
+    trm_ctor (tvsubst_trm_pre \<rho>2 (map_trm_pre id id id id snd snd y))"
+  apply unfold_locales
+      apply (unfold IImsupp_1_trm_def IImsupp_typ_def IImsupp_2_trm_def comp_def)[2]
+      apply (rule Un_bound UN_bound f_prems trm.FVars_bd_UNIVs typ.FVars_bd_UNIVs cmin_greater card_of_Card_order)+
+
+  subgoal for f1 f2 y
+    apply (subst trm_pre.map_comp, (assumption | rule supp_id_bound bij_id ordLess_ordLeq_trans cmin1 cmin2 card_of_Card_order)+)+
+    apply (unfold id_o_commute[of f1] id_o_commute[of f2] Product_Type.fst_comp_map_prod Product_Type.snd_comp_map_prod)
+    apply (subst trm_pre.map_comp[symmetric], (assumption | rule supp_id_bound bij_id ordLess_ordLeq_trans cmin1 cmin2 card_of_Card_order)+)+
+    apply (subst trm.permute_ctor[symmetric] isVVr_permute, (assumption | rule ordLess_ordLeq_trans cmin1 cmin2 card_of_Card_order)+)+
+
+    apply (rule case_split)
+     apply (subst if_P)
+      apply assumption
+     apply (unfold if_P if_not_P)
+     apply (unfold isVVr_def)[1]
+     apply (erule exE)
+     apply (rotate_tac -1)
+     apply (erule subst[OF sym])
+     apply (subst permute_VVr)
+         apply (assumption | rule ordLess_ordLeq_trans cmin1 cmin2 card_of_Card_order)+
+     apply (unfold asVVr_VVr)[1]
+     apply (rule IImsupp_permute_commute[THEN fun_cong, unfolded comp_def])
+          apply (assumption | rule ordLess_ordLeq_trans cmin1 cmin2 card_of_Card_order)+
+      apply (erule Int_subset_empty2, rule subsetI, (erule UnI1 UnI2 | assumption)+)
+
+    apply (rule trans)
+     apply (rule trm.permute_ctor)
+        apply (assumption | rule ordLess_ordLeq_trans cmin1 cmin2 card_of_Card_order)+
+    apply (subst map_subst)
+      apply (rule f_prems bij_id)+
+
+    apply (subst trm_pre.map_comp, (assumption | rule supp_id_bound bij_id ordLess_ordLeq_trans cmin1 cmin2 card_of_Card_order)+)+
+    apply (unfold id_o o_id)
+    apply (unfold comp_def)
+    apply (rule arg_cong[of _ _ trm_ctor])
+
+    apply (unfold tvsubst_trm_pre_def map_trm_pre_def comp_def typ.map_id0 Abs_trm_pre_inverse[OF UNIV_I])
+    apply (frule ordLess_ordLeq_trans)
+     apply (rule cmin1 card_of_Card_order)+
+    apply (rotate_tac -3)
+    apply (unfold typ.vvsubst_permute)
+    using typ.SSupp_natural[of f1 \<rho>2] SSupp_typ_TyVar_comp[of f1]
+      SSupp_typ_tvsubst_typ_bound[of "TyVar o f1" \<rho>2] f_prems(1) ordLess_ordLeq_trans[OF f_prems(2) cmin1[OF card_of_Card_order card_of_Card_order]]
+      SSupp_typ_tvsubst_typ_bound[of "permute_typ f1 o \<rho>2 o inv f1" "TyVar o f1"]
+    apply (auto split: sum.splits simp: Abs_trm_pre_inject trans[OF comp_apply[symmetric] typ.tvsubst_permutes[THEN fun_cong]] comp_def
+        ordLeq_ordLess_trans[OF card_of_image] typ.FVars_permute tvsubst_pat_comp
+        vvsubst_pat_tvsubst_pat intro!: tvsubst_typ_cong IImsupp_permute_commute[THEN fun_cong, unfolded comp_def]
+        typ.IImsupp_permute_commute[THEN fun_cong, unfolded comp_def] tvsubst_pat_cong)
+        apply auto
+     apply (auto simp: permute_typ_eq_tvsubst_typ_TyVar o_def vvsubst_typ_tvsubst_typ[unfolded comp_def, symmetric]
+        intro!: tvsubst_pat_cong typ.SSupp_comp_bound[unfolded comp_def])
+    apply (unfold typ.vvsubst_permute)
+    apply (auto intro!: typ.IImsupp_permute_commute[THEN fun_cong, unfolded comp_def])
+    done
+
+  subgoal premises prems
+    apply (rule case_split)
+     apply (subst if_P)
+      apply assumption
+     apply (unfold isVVr_def)[1]
+     apply (erule exE)
+     apply (drule sym)
+    apply (erule subst)
+     apply (unfold asVVr_VVr)
+     apply (rule case_split[of "_ = _"])
+      apply (rule iffD2[OF arg_cong2[OF _ refl, of _ _ "(\<subseteq>)"]])
+       apply (rule arg_cong[of _ _ FTVars])
+       apply assumption
+      apply (rule Un_upper1)
+     apply (rule subsetI)
+     apply (rule UnI2)
+     apply (unfold IImsupp_1_trm_def SSupp_trm_def tvVVr_tvsubst_trm_def tv\<eta>_trm_tvsubst_trm_def VVr_def[symmetric] image_comp[unfolded comp_def])[1]
+     apply (unfold comp_def)[1]
+     apply (rule UnI1)
+     apply (rule UN_I)
+      apply (rule CollectI)
+      apply assumption
+     apply assumption
+    apply (unfold if_not_P)
+    apply (erule thin_rl)
+
+    apply (unfold prod.collapse trm.FVars_ctor sets_tvsubst_trm_pre)
+    apply (subst map_subst)
+      apply (rule f_prems)
+    apply (rule bij_id)
+    apply (subst trm_pre.set_map, (rule bij_id supp_id_bound)+)+
+    apply (unfold image_id image_comp comp_def prod.collapse)
+    apply (rule Un_mono')+
+    subgoal
+      apply (unfold set1_trm_pre_def tvsubst_trm_pre_def UN_empty
+        sum.set_map UN_single UN_singleton UN_empty2 Un_empty_right Un_empty_left prod.set_map tvsubst_trm_pre_def
+        comp_def Abs_trm_pre_inverse[OF UNIV_I] IImsupp_1_trm_def IImsupp_typ_def SSupp_typ_def fst_conv snd_conv
+        tvVVr_tvsubst_typ_def tv\<eta>_typ_tvsubst_typ_def TyVar_def[symmetric] map_trm_pre_def typ.map_id0
+        SSupp_trm_def tvVVr_tvsubst_trm_def tv\<eta>_trm_tvsubst_trm_def VVr_def[symmetric] typ.set_map
+      )
+      using f_prems apply (auto split: sum.splits simp: FVars_tvsubst_typ_cmin)
+        apply (metis singletonD typ.set(1))
+        apply (metis singletonD typ.set(1))
+       apply (metis singletonD typ.set(1))
+      apply (subst (asm) PTVars_tvsubst_pat; (auto intro: ordLess_ordLeq_trans[OF _ cmin1])?)
+       apply (metis singletonD typ.set(1))
+      done
+    apply (rule iffD2[OF arg_cong2[OF refl, of _ _ "(\<subseteq>)"]])
+      apply (rule Diff_Un_disjunct)
+      apply (rule prems)
+     apply (rule Diff_mono[OF _ subset_refl])
+     apply (unfold UN_extend_simps(2))
+      (* REPEAT_DETERM *)
+     apply (rule subset_If)
+      apply (unfold UN_empty')[1]
+      apply (rule empty_subsetI)
+     apply (rule UN_mono[OF subset_refl])
+     apply (rule prems)
+     apply (unfold prod.collapse)
+     apply (erule UnI2 UnI1)
+    (* repeated *)
+     apply (rule subset_If)
+      apply (unfold UN_empty')[1]
+      apply (rule empty_subsetI)
+     apply (rule UN_mono[OF subset_refl])
+     apply (rule prems)
+     apply (unfold prod.collapse)
+     apply (erule UnI2 UnI1)
+    (* END REPEAT_DETERM *)
+    done
+
+    subgoal premises prems
+    apply (rule case_split)
+     apply (subst if_P)
+      apply assumption
+     apply (unfold isVVr_def)[1]
+     apply (erule exE)
+     apply (drule sym)
+    apply (erule subst)
+     apply (unfold asVVr_VVr)
+     apply (rule case_split[of "_ = _"])
+      apply (rule iffD2[OF arg_cong2[OF _ refl, of _ _ "(\<subseteq>)"]])
+       apply (rule arg_cong[of _ _ FVars])
+       apply assumption
+      apply (rule Un_upper1)
+     apply (rule subsetI)
+     apply (rule UnI2)
+     apply (unfold IImsupp_2_trm_def SSupp_trm_def tvVVr_tvsubst_trm_def tv\<eta>_trm_tvsubst_trm_def VVr_def[symmetric] image_comp[unfolded comp_def])[1]
+    apply (rule UnI2)
+     apply (rule UN_I)
+      apply (rule CollectI)
+      apply assumption
+     apply (unfold comp_def)[1]
+     apply assumption
+    apply (unfold if_not_P)
+    apply (erule thin_rl)
+
+    apply (unfold trm.FVars_ctor prod.collapse sets_tvsubst_trm_pre map_subst)
+    apply (subst trm_pre.set_map, (rule bij_id supp_id_bound)+)+
+    apply (unfold image_id image_comp comp_def prod.collapse sets_tvsubst_trm_pre)
+    apply (rule Un_mono')+
+      apply (rule Un_upper1)
+    apply (rule iffD2[OF arg_cong2[OF refl, of _ _ "(\<subseteq>)"]])
+      apply (rule Diff_Un_disjunct)
+      apply (rule prems)
+     apply (rule Diff_mono[OF _ subset_refl])
+     apply (unfold UN_extend_simps(2))
+      (* REPEAT_DETERM *)
+     apply (rule subset_If)
+      apply (unfold UN_empty')[1]
+      apply (rule empty_subsetI)
+     apply (rule UN_mono[OF subset_refl])
+     apply (rule prems)
+     apply (unfold prod.collapse)
+     apply (erule UnI2 UnI1)
+    (* repeated *)
+     apply (rule subset_If)
+      apply (unfold UN_empty')[1]
+      apply (rule empty_subsetI)
+     apply (rule UN_mono[OF subset_refl])
+     apply (rule prems)
+     apply (unfold prod.collapse)
+     apply (erule UnI2 UnI1)
+    (* END REPEAT_DETERM *)
+    done
+  done
+
+definition tvsubst :: "('tv, 'v) trm \<Rightarrow> ('tv, 'v) trm" where
+  "tvsubst \<equiv> tvsubst.REC_trm"
+
+lemma tvsubst_VVr: "tvsubst (VVr a :: ('tv::var, 'v::var) trm) = \<rho>1 a"
   apply (unfold tvsubst_def VVr_def comp_def)
   apply (rule trans)
-   apply (rule trm.rec_Uctor)
-      apply (unfold valid_P_def prod.case)
-      apply (rule conjI assms)+
-     apply (unfold eta_set_empties noclash_trm_def Uctor_def Un_empty prod.case)
+   apply (rule tvsubst.REC_ctor)
+     apply (unfold eta_set_empties noclash_trm_def Un_empty)
      apply (rule Int_empty_left conjI)+
   apply (subst trm_pre.map_comp, (rule supp_id_bound bij_id)+)+
   apply (unfold id_o o_id comp_def[of fst] fst_conv id_def[symmetric] trm_pre.map_id)
@@ -842,29 +575,23 @@ lemma tvsubst_VVr:
 
 lemma tvsubst_not_is_VVr:
   fixes x::"('tv::var, 'v::var) U1_pre"
-  assumes f_prems: "|SSupp_trm f1| <o cmin |UNIV::'tv set| |UNIV::'v set|" "|SSupp_typ f2| <o cmin |UNIV::'tv set| |UNIV::'v set|"
-    and empty_prems: "set3_trm_pre x \<inter> (IImsupp_1_trm f1 \<union> IImsupp_typ f2) = {}" "set4_trm_pre x \<inter> IImsupp_2_trm f1 = {}"
+  assumes empty_prems: "set3_trm_pre x \<inter> (IImsupp_1_trm \<rho>1 \<union> IImsupp_typ \<rho>2) = {}" "set4_trm_pre x \<inter> IImsupp_2_trm \<rho>1 = {}"
     and noclash: "noclash_trm x"
     and VVr_prems: "\<not>isVVr (trm_ctor x)"
   shows
-    "tvsubst f1 f2 (trm_ctor x) = trm_ctor (tvsubst_trm_pre f2 (map_trm_pre id id id id (tvsubst f1 f2) (tvsubst f1 f2) x))"
+    "tvsubst (trm_ctor x) = trm_ctor (tvsubst_trm_pre \<rho>2 (map_trm_pre id id id id tvsubst tvsubst x))"
   apply (unfold tvsubst_def)
-  apply (subgoal_tac "valid_P (f1, f2)")
-   prefer 2
-   apply (unfold valid_P_def prod.case)[1]
-   apply (rule conjI f_prems)+
   apply (rule trans)
-   apply (rule trm.rec_Uctor)
-      apply assumption
-     apply (unfold PFVars_1_def PFVars_2_def prod.case)
+   apply (rule tvsubst.REC_ctor)
      apply (rule empty_prems noclash)+
-  apply (unfold Uctor_def prod.case)
   apply (subst trm_pre.map_comp, (rule supp_id_bound bij_id)+)+
   apply (unfold id_o o_id comp_def[of fst] fst_conv id_def[symmetric] trm_pre.map_id)
   apply (subst if_not_P, rule VVr_prems)+
   apply (unfold comp_def snd_conv if_P)
   apply (rule refl)
   done
+
+end
 
 lemma tvsubst_simps[simp]:
   fixes f1::"'v \<Rightarrow> ('tv::var, 'v::var) trm" and f2::"'tv \<Rightarrow> 'tv typ"
